\documentclass[aps,12pt]{revtex4}
\usepackage[a4paper]{geometry}
\usepackage{graphicx}
\usepackage{amssymb,amsfonts,amsmath,amsthm}
\usepackage{bm}
\usepackage{pslatex}
\usepackage{mathptmx}
\usepackage{bookman}
\usepackage{chemarr}

 	 
\begin{document}

\section{Equilibrium $[0,1]$}
\begin{equation}
	\xrightleftharpoons[]{} A, \;\; \Gamma = K - [A]
\end{equation}
Starting from $[A]$, the extent $x$ is:
\begin{equation}
	x = K-[A] = \Gamma
\end{equation}
The solution is
\begin{equation}
	[A] = K
\end{equation}

\section{Equilibrium $[1,0]$}
\begin{equation}
	A \xrightleftharpoons[]{} , \;\; \Gamma = K[A]-1
\end{equation}
Starting from $[A]$, the extent $x$ is:
\begin{equation}
	x = \dfrac{K[A]-1}{K} = \dfrac{\Gamma}{K}
\end{equation}
The solution is
\begin{equation}
	[A] = 1/K
\end{equation}


\section{Equilibrium $[0,2]$}
\begin{equation}
	\xrightleftharpoons[]{} 2A, \;\; \Gamma = K - [A]^n
\end{equation}
Starting from $[A]$, the extent $x$ is:
\begin{equation}
	x = \dfrac{\sqrt{K}-[A]}{2}
\end{equation}
The solution is
\begin{equation}
	[A] = \sqrt{K}
\end{equation}

\section{Equilibrium $[0,n]$}
\begin{equation}
	\xrightleftharpoons[]{} nA, \;\; \Gamma = K - [A]^n
\end{equation}
Starting from $[A]$, the extent $x$ is:
\begin{equation}
	x = \dfrac{ K^{1/n}-[A]}{n}
\end{equation}
The solution is
\begin{equation}
	[A] = K^{1/n}
\end{equation}


\section{Equilibrium $[1,1]$}
\begin{equation}
	A \xrightleftharpoons[]{} B, \;\; \Gamma = K[A]-[B]
\end{equation}
Starting from $[A],[B]$, the extent $x$ is:
\begin{equation}
	x = \dfrac{K[A]-[B]}{1+K}
\end{equation}
The solution is:
\begin{equation}
	[A] = \dfrac{[A]+[B]}{1+K}, \; [B] = K \dfrac{ [A]+[B] }{1+K}
\end{equation}


\section{Equilibrium $[0,[1,1]]$}
\begin{equation}
	\xrightleftharpoons[]{} A+B, \;\; \Gamma = K - [A][B]
\end{equation}
Starting from $[A],[B]$, the extent $x$ is solution of:
\begin{equation}
	K = ([A]+x)([B]+x) = x^2 + ([A]+[B])x + [A][B]
\end{equation}
Using:
\begin{equation}
	\Delta = 4K + ([A]-[B])^2 > 0
\end{equation}
we get:
\begin{equation}
	x = \dfrac{\sqrt{\Delta}-([A]+[B])}{2}
\end{equation}
The solution is
\begin{equation}
	[A] =  \dfrac{([A]-[B])+\sqrt{\Delta}}{2},\;\;[B] = \dfrac{\sqrt{\Delta}-([A]-[B])}{2}
\end{equation}

\section{Equilibrium $[1,[1,1]]$}
\begin{equation}
	A\xrightleftharpoons[]{} B+C, \;\; \Gamma = K[A] - [B][C]
\end{equation}
Starting from $[A],[B],[C]$, the extent $x$ is solution of:
\begin{equation}
	K([A]-x) = ([B]+x)([C]+x) = x^2 + ([B]+[C])x + [B][C]
\end{equation}
or
\begin{equation}
	x^2 + ([B]+[C]+K) x + [B][C]-K[A] = 0	
\end{equation}
With:
\begin{equation}
	\Delta = K^2 + ([B]-[C])^2 + 2K(2[A]+[B]+[C]) > 0
\end{equation}
the extent is:
\begin{equation}
	x = \dfrac{\sqrt{\Delta} - ([B]+[C]+K) }{2}
\end{equation}

\section{Equilibrium $[[1,1],[1,1]]$}
\begin{equation}
	A+B\xrightleftharpoons[]{} C+D, \;\; \Gamma = K[A][B] - [C][D]
\end{equation}
Starting from $[A],[B],[C],[D]$, the extent $x$ is solution of:
\begin{equation}
	K([A]-x)([B]-x) = ([C]+x)([D]+x) 
\end{equation}

\begin{equation}
	(K-1)x^2 - ( K([A]+[B]) + ([C]+[D])) x + (K[A][B] - [C][D]) = 0
\end{equation}
The discriminant is:
\begin{equation}
	\Delta = ([C]-[D])^2 + K \left[ K([A]-[B])^2 + 2(([A]+[B])([C]+[D]))+4([A][B]+[C][D]) \right] \geq 0
\end{equation}

\begin{equation}
x = 2 \dfrac{K[A][B]-[C][D]}{ K([A]+[B]) + ([C]+[D])) + \sqrt{\Delta} }
\end{equation}




\end{document}