\documentclass[aps,11pt]{revtex4}
\usepackage{graphicx}
\usepackage{amssymb,amsfonts,amsmath,amsthm}
\usepackage{chemarr}
\usepackage{bm}
\usepackage{pslatex}
\usepackage{xfrac}
\usepackage{hyperref}


\begin{document}
\title{Diffusion}
\maketitle

\section{Evaluation}

\subsection{Bulk}
We have $C_{i}$ at $x_i$ for $i\in[1:N]$.
For $x\in[x_{i-1},x_{i+1}]$:
\begin{equation}
\left\lbrace
\begin{array}{rcl}
	C(x)    & = & C_i + \alpha_i (x-x_i) + \frac{1}{2}\beta_i (x-x_i)^2\\
	C_{i-1} & = & C_i + \alpha_i (x_{i-1}-x_{i} ) + \frac{1}{2}\beta_i (x_{i-1}-x_i)^2\\
    C_{i+1} & = & C_i + \alpha_i (x_{i+1}-x_{i} ) + \frac{1}{2}\beta_i (x_{i+1}-x_i)^2\\
\end{array}
\right.
\end{equation}

$$
	\delta_{i_+} = (x_{i+1}-x_{i} ), \delta_{i_-} = (x_{i}-x_{i-1} ) 
$$
\begin{equation}
	\alpha_i = \dfrac{ \delta_{i_-}^2 C_{i+1}  +(\delta_{i_+}^2-\delta_{i_-}^2)C_i - \delta_{i_+}^2 C_{i-1} }{ \delta_{i_+}\delta_{i_-}(\delta_{i_+}+\delta_{i_-})  }
\end{equation}

\begin{equation}
\label{eq:beta_i}
	\beta_i = 2\dfrac{ \delta_{i_-} C_{i+1}  - (\delta_{i_+}+\delta_{i_-})C_i + \delta_{i_+} C_{i-1} }{ \delta_{i_+}\delta_{i_-}(\delta_{i_+}+\delta_{i_-})  }
\end{equation}

\subsection{Left}
\begin{equation}
\left\lbrace
\begin{array}{rcl}
	C(x)   & = & C_1 + \alpha_1 (x-x_1) + \frac{1}{2}\beta_1 (x-x_1)^2\\
	C_2    & = & C_1 + \alpha_1 (x_2-x_1) + \frac{1}{2}\beta_1 (x_2-x_1)^2 = C_1 + \alpha_1 \delta_{2_-} + \frac{1}{2}\beta_1 \delta_{2_-}^2 \\
	C_3    & = & C_1 + \alpha_1 (x_3-x_1) + \frac{1}{2}\beta_1 (x_3-x_1)^2 = C_1 + \alpha_1 (\delta_{2_-}+ \delta_{2_+} )+ \frac{1}{2}\beta_1 (\delta_{2_-}+ \delta_{2_+} )^2
\end{array}
\right.
\end{equation}

\begin{equation}
	\alpha_1 = \dfrac{ -\delta_{2_+}(\delta_{2_+}+2\delta_{2_-}) C_1 + (\delta_{2_+}+\delta_{2_-})^2  C_2 - \delta_{2_-}^2 C_3}{\delta_{2_+}\delta_{2_-}(\delta_{2_+}+\delta_{2_-})}
\end{equation}

\begin{equation}
	\alpha_1 = 0  \iff C_1 = \dfrac{ (\delta_{2_+}+\delta_{2_-})^2  C_2 - \delta_{2_-}^2 C_3}{\delta_{2_+}(\delta_{2_+}+2\delta_{2_-})}
\end{equation}

\subsection{Right}
\begin{equation}
\left\lbrace
\begin{array}{rcl}
	C(x)    & = & C_N + \alpha_N (x-x_N) + \frac{1}{2}\beta_N (x-x_N)^2\\
	C_{N-1} & = & C_N + \alpha_N (x_{N-1}-x_{N}) +  \frac{1}{2}\beta_N (x_{N-1}-x_{N}) ^2 = C_N - \alpha_N {\delta_{N_{1+}}} +  \frac{1}{2}\beta_N {\delta_{N_{1+}}}^2\\\
	C_{N-2} & = & C_N + \alpha_N (x_{N-2}-x_{N}) +  \frac{1}{2}\beta_N (x_{N-2}-x_{N}) ^2 = C_N - \alpha_N (\delta_{N_{1+}}+\delta_{N_{1-}}) + \frac{1}{2}\beta_N (\delta_{N_{1+}}+\delta_{N_{1-}})^2\\
\end{array}
\right.
\end{equation}

\begin{equation}
	\alpha_N = \dfrac{\delta_{N_{1+}}^2C_{N-2} - (\delta_{N_{1+}}+\delta_{N_{1-}})^2 C_{N-1} + \delta_{N_{1-}}(2\delta_{N_{1-}}+\delta_{N_{1+}}) C_N }{(\delta_{N_{1+}}+\delta_{N_{1-}})\delta_{N_{1+}}\delta_{N_{1-}}}
\end{equation}

\begin{equation}
	\alpha_N = 0 \iff C_N = \dfrac{(\delta_{N_{1+}}+\delta_{N_{1-}})^2 C_{N-1} - \delta_{N_{1+}}^2C_{N-2}}{\delta_{N_{1-}}(2\delta_{N_{1-}}+\delta_{N_{1+}}) }
\end{equation}

\subsection{Scheme}

\begin{equation}
C_1(t) = f(t), \partial_x C_N = 0
\end{equation}	

\begin{equation}
\forall 1<i<N, \; \dfrac{C_i^{n+1}-C_i^{n}}{\delta t} = \dfrac{D}{2} \left[ \beta_i^{n+1} + \beta_i^{n}\right]
\end{equation}

\begin{equation}
\forall 1<i<N, \;  C_i^{n+1} - \dfrac{D\delta t}{2} \beta_i^{n+1} = C_i^{n} +  \dfrac{D\delta t}{2} \beta_i^{n}
\end{equation}
using \eqref{eq:beta_i}

$$
		\beta_i = 2\dfrac{ \delta_{i_-} C_{i+1}  - (\delta_{i_+}+\delta_{i_-})C_i + \delta_{i_+} C_{i-1} }{ \delta_{i_+}\delta_{i_-}(\delta_{i_+}+\delta_{i_-})  }
$$

\begin{equation}
\begin{array}{rl}
\forall 1<i<N, &  
- \dfrac{D\delta t}{\delta_{i_-}(\delta_{i_+}+\delta_{i_-})} C_{i-1}^{n+1} + \left[1+\dfrac{D\delta t}{\delta_{i_+}\delta_{i_-}}\right] C_i^{n+1} - \dfrac{D\delta t}{\delta_{i_+}(\delta_{i_+}+\delta_{i_-})}C_{i+1}^{n+1}\\
\\
 = & C_i^{n} +  \dfrac{D\delta t}{2} \beta_i^{n}\\
 \\
 = & \dfrac{D\delta t}{\delta_{i_-}(\delta_{i_+}+\delta_{i_-})} C_{i-1}^{n} 
 +\left[1-\dfrac{D\delta t}{\delta_{i_+}\delta_{i_-}}\right] C_i^{n}
 +\dfrac{D\delta t}{\delta_{i_+}(\delta_{i_+}+\delta_{i_-})}C_{i+1}^{n}\\
 \end{array}
 \end{equation}

\begin{equation}
	\gamma = \dfrac{D\delta t}{\bar{\delta}^2}
\end{equation}

\begin{equation}
\begin{array}{rl}
 & - \gamma\dfrac{\bar{\delta}^2}{\delta_{i_-}(\delta_{i_+}+\delta_{i_-})} C_{i-1}^{n+1} + \left[1+\gamma\dfrac{\bar{\delta}^2}{\delta_{i_+}\delta_{i_-}}\right] C_i^{n+1} - \gamma\dfrac{\bar{\delta}^2}{\delta_{i_+}(\delta_{i_+}+\delta_{i_-})}C_{i+1}^{n+1}\\
 \\
 = & \gamma\dfrac{\bar{\delta}^2}{\delta_{i_-}(\delta_{i_+}+\delta_{i_-})} C_{i-1}^{n} 
 +\left[1-\gamma\dfrac{\bar{\delta}^2}{\delta_{i_+}\delta_{i_-}}\right] C_i^{n}
 +\gamma\dfrac{\bar{\delta}^2}{\delta_{i_+}(\delta_{i_+}+\delta_{i_-})}C_{i+1}^{n}\\
 \end{array}
\end{equation}

\begin{equation}
\left\lbrace
\begin{array}{rcc}
	a_i & = & \dfrac{\bar{\delta}^2}{\delta_{i_-}(\delta_{i_+}+\delta_{i_-})}\\
	\\
	b_i & = & \dfrac{\bar{\delta}^2}{\delta_{i_+}\delta_{i_-}}\\
	\\
	c_i & = & \dfrac{\bar{\delta}^2}{\delta_{i_+}(\delta_{i_+}+\delta_{i_-})}\\
\end{array}
\right.
\end{equation}

\subsection{Fixed Left, Right Wall}
\begin{equation}
\begin{bmatrix}
1 & \\
-\gamma a_i & 1+ \gamma b_i & \gamma c_i \\
            &               & \\
\end{bmatrix}
\end{equation}



\end{document}
