\documentclass[aps,12pt]{revtex4}
\usepackage[a4paper]{geometry}
\usepackage{graphicx}
\usepackage{amssymb,amsfonts,amsmath,amsthm}
\usepackage{bm}
\usepackage{pslatex}
\usepackage{mathptmx}


\begin{document}

\section{Normal}

$$ax^2+bx+c=0$$

$$
\Delta = b^2-4ac > 0
$$	

$$
\left\lbrace
\begin{array}{rcl}
	x_- & = &  \dfrac{-b-\sqrt{\Delta}}{2a} \\
	\\
	& = & -  \dfrac{b+\sqrt{\Delta}}{2a} \\
	\\
	& = & -  \dfrac{(b+\sqrt{\Delta})(b-\sqrt{\Delta})}{2a(b-\sqrt{\Delta})}\\
	\\
	& = & - \dfrac{b^2-\Delta}{2a(b-\sqrt{\Delta})}\\
	\\
	& = & (-c) \dfrac{2}{b-\sqrt{\Delta}} \\ 
\end{array}
\right.
$$

$$
\left\lbrace
\begin{array}{rcl}
	x_+ & = &  \dfrac{-b+\sqrt{\Delta}}{2a} \\
	\\
	 & = & \dfrac{(\sqrt{\Delta}-b)(\sqrt{\Delta}+b)}{2a(\sqrt{\Delta}+b)}\\
	\\
	& = & \dfrac{\Delta-b^2}{2a(\sqrt{\Delta}+b)}\\
	\\
	& = & (-c) \dfrac{2}{\sqrt{\Delta}+b}\\
\end{array}
\right.
$$


\section{Reduced}

$$ax^2+2b'x+c=0$$

$$
\Delta' = b'^2-ac > 0
$$	

$$
	x_-' = \dfrac{-b'-\sqrt{\Delta'}}{a} = \dfrac{1}{\sqrt{\Delta'}-b'}{c}
$$

$$
	x_+' = \dfrac{-b'+\sqrt{\Delta'}}{a} = \dfrac{-1}{\sqrt{\Delta'}+b'}{c}
$$

\end{document}